examples/lean_chacha20/proofs/lean/extraction/lean_chacha20_manual_edit.lean
@@ -1,5 +1,6 @@
+
 -- Experimental lean backend for Hax
--- Lib.lean can be found in hax/proof-libs/lean :
+-- The Hax prelude library can be found in hax/proof-libs/lean
 import Hax
 import Std.Tactic.Do
 import Std.Do.Triple
@@ -10,415 +11,418 @@ open Std.Tactic
 set_option mvcgen.warning false
 set_option linter.unusedVariables false
 
-def hacspec_helper_to_le_u32s_3 (bytes : (Array u8))
-  : Result (Vector u32 3) := do
-  let (out : (Vector u32 3)) ← pure (← hax_repeat 0 3);
-  let (out : (Vector u32 3)) ← pure
-    (← hax_folds_fold_range
+def hacspec_helper.to_le_u32s_3 (bytes : (RustSlice UInt8))
+  : Result (RustArray UInt32 3) := do
+  let (out : (RustArray UInt32 3)) ← pure (← hax.repeat 0 3);
+  let (out : (RustArray UInt32 3)) ← pure
+    (← hax.folds.fold_range
     0
       3
-      (fun (out : (Vector u32 3)) (_ : usize)=> do true)
+      (fun (out : (RustArray UInt32 3)) (_ : USize) => do true)
       out
-      (fun (out : (Vector u32 3)) (i : usize)=> do
-        (← hax_monomorphized_update_at_update_at_usize
+      (fun (out : (RustArray UInt32 3)) (i : USize) => do
+        (← hax.monomorphized_update_at.update_at_usize
         out
           i
-          (← num__8_impl_from_le_bytes
-          (← result_impl_unwrap (Vector u8 4) array_TryFromSliceError
-            (← convert_TryInto_try_into
-              (← ops_index_Index_index
+          (← num._8_impl.from_le_bytes
+          (← result.impl.unwrap (RustArray UInt8 4) array.TryFromSliceError
+            (← convert.TryInto.try_into
+              (← ops.index.Index.index
                 bytes
-                  (constr_ops_range_Range
-                    (ops_range_Range_start := (← hax_machine_int_mul 4 i))
-                    (ops_range_Range_end := (← (← hax_machine_int_mul 4 i) +?
-                    4))))))))));
+                  (ops.range.Range.mk
+                  (_start := (← 4 *? i)) (_end := (← (← 4 *? i) +? 4))))))))));
   out
 
-def hacspec_helper_to_le_u32s_8 (bytes : (Array u8))
-  : Result (Vector u32 8) := do
-  let (out : (Vector u32 8)) ← pure (← hax_repeat 0 8);
-  let (out : (Vector u32 8)) ← pure
-    (← hax_folds_fold_range
+def hacspec_helper.to_le_u32s_8 (bytes : (RustSlice UInt8))
+  : Result (RustArray UInt32 8) := do
+  let (out : (RustArray UInt32 8)) ← pure (← hax.repeat 0 8);
+  let (out : (RustArray UInt32 8)) ← pure
+    (← hax.folds.fold_range
     0
       8
-      (fun (out : (Vector u32 8)) (_ : usize)=> do true)
+      (fun (out : (RustArray UInt32 8)) (_ : USize) => do true)
       out
-      (fun (out : (Vector u32 8)) (i : usize)=> do
-        (← hax_monomorphized_update_at_update_at_usize
+      (fun (out : (RustArray UInt32 8)) (i : USize) => do
+        (← hax.monomorphized_update_at.update_at_usize
         out
           i
-          (← num__8_impl_from_le_bytes
-          (← result_impl_unwrap (Vector u8 4) array_TryFromSliceError
-            (← convert_TryInto_try_into
-              (← ops_index_Index_index
+          (← num._8_impl.from_le_bytes
+          (← result.impl.unwrap (RustArray UInt8 4) array.TryFromSliceError
+            (← convert.TryInto.try_into
+              (← ops.index.Index.index
                 bytes
-                  (constr_ops_range_Range
-                    (ops_range_Range_start := (← hax_machine_int_mul 4 i))
-                    (ops_range_Range_end := (← (← hax_machine_int_mul 4 i) +?
-                    4))))))))));
+                  (ops.range.Range.mk
+                  (_start := (← 4 *? i)) (_end := (← (← 4 *? i) +? 4))))))))));
   out
 
-def hacspec_helper_to_le_u32s_16 (bytes : (Array u8))
-  : Result (Vector u32 16) := do
-  let (out : (Vector u32 16)) ← pure (← hax_repeat 0 16);
-  let (out : (Vector u32 16)) ← pure
-    (← hax_folds_fold_range
+def hacspec_helper.to_le_u32s_16 (bytes : (RustSlice UInt8))
+  : Result (RustArray UInt32 16) := do
+  let (out : (RustArray UInt32 16)) ← pure (← hax.repeat 0 16);
+  let (out : (RustArray UInt32 16)) ← pure
+    (← hax.folds.fold_range
     0
       16
-      (fun (out : (Vector u32 16)) (_ : usize)=> do true)
+      (fun (out : (RustArray UInt32 16)) (_ : USize) => do true)
       out
-      (fun (out : (Vector u32 16)) (i : usize)=> do
-        (← hax_monomorphized_update_at_update_at_usize
+      (fun (out : (RustArray UInt32 16)) (i : USize) => do
+        (← hax.monomorphized_update_at.update_at_usize
         out
           i
-          (← num__8_impl_from_le_bytes
-          (← result_impl_unwrap (Vector u8 4) array_TryFromSliceError
-            (← convert_TryInto_try_into
-              (← ops_index_Index_index
+          (← num._8_impl.from_le_bytes
+          (← result.impl.unwrap (RustArray UInt8 4) array.TryFromSliceError
+            (← convert.TryInto.try_into
+              (← ops.index.Index.index
                 bytes
-                  (constr_ops_range_Range
-                    (ops_range_Range_start := (← hax_machine_int_mul 4 i))
-                    (ops_range_Range_end := (← (← hax_machine_int_mul 4 i) +?
-                    4))))))))));
+                  (ops.range.Range.mk
+                  (_start := (← 4 *? i)) (_end := (← (← 4 *? i) +? 4))))))))));
   out
 
-def hacspec_helper_u32s_to_le_bytes (state : (Vector u32 16))
-  : Result (Vector u8 64) := do
-  let (out : (Vector u8 64)) ← pure (← hax_repeat 0 64);
-  let (out : (Vector u8 64)) ← pure
-    (← hax_folds_fold_range
+def hacspec_helper.u32s_to_le_bytes (state : (RustArray UInt32 16))
+  : Result (RustArray UInt8 64) := do
+  let (out : (RustArray UInt8 64)) ← pure (← hax.repeat 0 64);
+  let (out : (RustArray UInt8 64)) ← pure
+    (← hax.folds.fold_range
     0
-      (← slice_impl_len u32 (← unsize state))
-      (fun (out : (Vector u8 64)) (_ : usize)=> do true)
+      (← slice.impl.len UInt32 (← unsize state))
+      (fun (out : (RustArray UInt8 64)) (_ : USize) => do true)
       out
-      (fun (out : (Vector u8 64)) (i : usize)=> do
-        let (tmp : (Vector u8 4)) ← pure
-          (← num__8_impl_to_le_bytes (← ops_index_Index_index state i));
-        (← hax_folds_fold_range
+      (fun (out : (RustArray UInt8 64)) (i : USize) => do
+        let (tmp : (RustArray UInt8 4)) ← pure
+          (← num._8_impl.to_le_bytes (← ops.index.Index.index state i));
+        (← hax.folds.fold_range
         0
           4
-          (fun (out : (Vector u8 64)) (_ : usize)=> do true)
+          (fun (out : (RustArray UInt8 64)) (_ : USize) => do true)
           out
-          (fun (out : (Vector u8 64)) (j : usize)=> do
-            (← hax_monomorphized_update_at_update_at_usize
+          (fun (out : (RustArray UInt8 64)) (j : USize) => do
+            (← hax.monomorphized_update_at.update_at_usize
             out
-              (← (← hax_machine_int_mul i 4) +? j)
-              (← ops_index_Index_index tmp j))))));
+              (← (← i *? 4) +? j)
+              (← ops.index.Index.index tmp j))))));
   out
 
-def hacspec_helper_xor_state (state : (Vector u32 16)) (other : (Vector u32 16))
-  : Result (Vector u32 16) := do
-  let (state : (Vector u32 16)) ← pure
-    (← hax_folds_fold_range
+def hacspec_helper.xor_state
+  (state : (RustArray UInt32 16)) (other : (RustArray UInt32 16))
+  : Result (RustArray UInt32 16) := do
+  let (state : (RustArray UInt32 16)) ← pure
+    (← hax.folds.fold_range
     0
       16
-      (fun (state : (Vector u32 16)) (_ : usize)=> do true)
+      (fun (state : (RustArray UInt32 16)) (_ : USize) => do true)
       state
-      (fun (state : (Vector u32 16)) (i : usize)=> do
-        (← hax_monomorphized_update_at_update_at_usize
+      (fun (state : (RustArray UInt32 16)) (i : USize) => do
+        (← hax.monomorphized_update_at.update_at_usize
         state
           i
-          (← hax_machine_int_bitxor
-          (← ops_index_Index_index state i)
-            (← ops_index_Index_index other i)))));
+          (← hax.machine_int.bitxor
+          (← ops.index.Index.index state i)
+            (← ops.index.Index.index other i)))));
   state
 
-def hacspec_helper_add_state (state : (Vector u32 16)) (other : (Vector u32 16))
-  : Result (Vector u32 16) := do
-  let (state : (Vector u32 16)) ← pure
-    (← hax_folds_fold_range
+def hacspec_helper.add_state
+  (state : (RustArray UInt32 16)) (other : (RustArray UInt32 16))
+  : Result (RustArray UInt32 16) := do
+  let (state : (RustArray UInt32 16)) ← pure
+    (← hax.folds.fold_range
     0
       16
-      (fun (state : (Vector u32 16)) (_ : usize)=> do true)
+      (fun (state : (RustArray UInt32 16)) (_ : USize) => do true)
       state
-      (fun (state : (Vector u32 16)) (i : usize)=> do
-        (← hax_monomorphized_update_at_update_at_usize
+      (fun (state : (RustArray UInt32 16)) (i : USize) => do
+        (← hax.monomorphized_update_at.update_at_usize
         state
           i
-          (← num__8_impl_wrapping_add
-          (← ops_index_Index_index state i)
-            (← ops_index_Index_index other i)))));
+          (← num._8_impl.wrapping_add
+          (← ops.index.Index.index state i)
+            (← ops.index.Index.index other i)))));
   state
 
-def hacspec_helper_update_array (array : (Vector u8 64)) (val : (Array u8))
-  : Result (Vector u8 64) := do
-  let (_ : hax_Tuple0) ← pure
-    (← assert (← hax_machine_int_ge 64 (← slice_impl_len u8 val)));
-  let (array : (Vector u8 64)) ← pure
-    (← hax_folds_fold_range
+def hacspec_helper.update_array
+  (array : (RustArray UInt8 64)) (val : (RustSlice UInt8))
+  : Result (RustArray UInt8 64) := do
+  let (_ : hax.Tuple0) ← pure
+    (← assert (← hax.machine_int.ge 64 (← slice.impl.len UInt8 val)));
+  let (array : (RustArray UInt8 64)) ← pure
+    (← hax.folds.fold_range
     0
-      (← slice_impl_len u8 val)
-      (fun (array : (Vector u8 64)) (_ : usize)=> do true)
+      (← slice.impl.len UInt8 val)
+      (fun (array : (RustArray UInt8 64)) (_ : USize) => do true)
       array
-      (fun (array : (Vector u8 64)) (i : usize)=> do
-        (← hax_monomorphized_update_at_update_at_usize
+      (fun (array : (RustArray UInt8 64)) (i : USize) => do
+        (← hax.monomorphized_update_at.update_at_usize
         array
           i
-          (← ops_index_Index_index val i))));
+          (← ops.index.Index.index val i))));
   array
 
-abbrev State := (Vector u32 16)
-abbrev Block := (Vector u8 64)
-abbrev ChaChaIV := (Vector u8 12)
-abbrev ChaChaKey := (Vector u8 32)
-abbrev StateIdx := (hax__autogenerated_refinement__BoundedUsize_BoundedUsize 0
+abbrev State := (RustArray UInt32 16)
+
+abbrev Block := (RustArray UInt8 64)
+
+abbrev ChaChaIV := (RustArray UInt8 12)
+
+abbrev ChaChaKey := (RustArray UInt8 32)
+
+abbrev StateIdx := (hax__autogenerated_refinement__BoundedUsize.BoundedUsize 0
 15)
+
 def chacha20_line
-    (a : (hax__autogenerated_refinement__BoundedUsize_BoundedUsize 0 15)) (b :
-    (hax__autogenerated_refinement__BoundedUsize_BoundedUsize 0 15)) (d :
-    (hax__autogenerated_refinement__BoundedUsize_BoundedUsize 0 15)) (s : u32)
-    (m : (Vector u32 16)) : Result (Vector u32 16) := do
-  let (state : (Vector u32 16)) ← pure m;
-  let (state : (Vector u32 16)) ← pure
-    (← hax_update_at
+  (a : (hax__autogenerated_refinement__BoundedUsize.BoundedUsize 0 15)) (b :
+  (hax__autogenerated_refinement__BoundedUsize.BoundedUsize 0 15)) (d :
+  (hax__autogenerated_refinement__BoundedUsize.BoundedUsize 0 15)) (s : UInt32)
+  (m : (RustArray UInt32 16)) : Result (RustArray UInt32 16) := do
+  let (state : (RustArray UInt32 16)) ← pure m;
+  let (state : (RustArray UInt32 16)) ← pure
+    (← hax.update_at
     state
       a
-      (← num__8_impl_wrapping_add
-      (← ops_index_Index_index state a)
-        (← ops_index_Index_index state b)));
-  let (state : (Vector u32 16)) ← pure
-    (← hax_update_at
+      (← num._8_impl.wrapping_add
+      (← ops.index.Index.index state a)
+        (← ops.index.Index.index state b)));
+  let (state : (RustArray UInt32 16)) ← pure
+    (← hax.update_at
     state
       d
-      (← hax_machine_int_bitxor
-      (← ops_index_Index_index state d)
-        (← ops_index_Index_index state a)));
-  let (state : (Vector u32 16)) ← pure
-    (← hax_update_at
+      (← hax.machine_int.bitxor
+      (← ops.index.Index.index state d)
+        (← ops.index.Index.index state a)));
+  let (state : (RustArray UInt32 16)) ← pure
+    (← hax.update_at
     state
       d
-      (← num__8_impl_rotate_left (← ops_index_Index_index state d) s));
+      (← num._8_impl.rotate_left (← ops.index.Index.index state d) s));
   state
 
 def chacha20_quarter_round
-    (a : (hax__autogenerated_refinement__BoundedUsize_BoundedUsize 0 15)) (b :
-    (hax__autogenerated_refinement__BoundedUsize_BoundedUsize 0 15)) (c :
-    (hax__autogenerated_refinement__BoundedUsize_BoundedUsize 0 15)) (d :
-    (hax__autogenerated_refinement__BoundedUsize_BoundedUsize 0 15)) (state :
-    (Vector u32 16)) : Result (Vector u32 16) := do
-  let (state : (Vector u32 16)) ← pure (← chacha20_line a b d 16 state);
-  let (state : (Vector u32 16)) ← pure (← chacha20_line c d b 12 state);
-  let (state : (Vector u32 16)) ← pure (← chacha20_line a b d 8 state);
+  (a : (hax__autogenerated_refinement__BoundedUsize.BoundedUsize 0 15)) (b :
+  (hax__autogenerated_refinement__BoundedUsize.BoundedUsize 0 15)) (c :
+  (hax__autogenerated_refinement__BoundedUsize.BoundedUsize 0 15)) (d :
+  (hax__autogenerated_refinement__BoundedUsize.BoundedUsize 0 15)) (state :
+  (RustArray UInt32 16)) : Result (RustArray UInt32 16) := do
+  let (state : (RustArray UInt32 16)) ← pure (← chacha20_line a b d 16 state);
+  let (state : (RustArray UInt32 16)) ← pure (← chacha20_line c d b 12 state);
+  let (state : (RustArray UInt32 16)) ← pure (← chacha20_line a b d 8 state);
   (← chacha20_line c d b 7 state)
 
-def chacha20_double_round (state : (Vector u32 16))
-  : Result (Vector u32 16) := do
-  let (state : (Vector u32 16)) ← pure
+def chacha20_double_round (state : (RustArray UInt32 16))
+  : Result (RustArray UInt32 16) := do
+  let (state : (RustArray UInt32 16)) ← pure
     (← chacha20_quarter_round
-    (0 : (hax__autogenerated_refinement__BoundedUsize_BoundedUsize 0 15))
-      (4 : (hax__autogenerated_refinement__BoundedUsize_BoundedUsize 0 15))
-      (8 : (hax__autogenerated_refinement__BoundedUsize_BoundedUsize 0 15))
-      (12 : (hax__autogenerated_refinement__BoundedUsize_BoundedUsize 0 15))
+    (0 : (hax__autogenerated_refinement__BoundedUsize.BoundedUsize 0 15))
+      (4 : (hax__autogenerated_refinement__BoundedUsize.BoundedUsize 0 15))
+      (8 : (hax__autogenerated_refinement__BoundedUsize.BoundedUsize 0 15))
+      (12 : (hax__autogenerated_refinement__BoundedUsize.BoundedUsize 0 15))
       state);
-  let (state : (Vector u32 16)) ← pure
+  let (state : (RustArray UInt32 16)) ← pure
     (← chacha20_quarter_round
-    (1 : (hax__autogenerated_refinement__BoundedUsize_BoundedUsize 0 15))
-      (5 : (hax__autogenerated_refinement__BoundedUsize_BoundedUsize 0 15))
-      (9 : (hax__autogenerated_refinement__BoundedUsize_BoundedUsize 0 15))
-      (13 : (hax__autogenerated_refinement__BoundedUsize_BoundedUsize 0 15))
+    (1 : (hax__autogenerated_refinement__BoundedUsize.BoundedUsize 0 15))
+      (5 : (hax__autogenerated_refinement__BoundedUsize.BoundedUsize 0 15))
+      (9 : (hax__autogenerated_refinement__BoundedUsize.BoundedUsize 0 15))
+      (13 : (hax__autogenerated_refinement__BoundedUsize.BoundedUsize 0 15))
       state);
-  let (state : (Vector u32 16)) ← pure
+  let (state : (RustArray UInt32 16)) ← pure
     (← chacha20_quarter_round
-    (2 : (hax__autogenerated_refinement__BoundedUsize_BoundedUsize 0 15))
-      (6 : (hax__autogenerated_refinement__BoundedUsize_BoundedUsize 0 15))
-      (10 : (hax__autogenerated_refinement__BoundedUsize_BoundedUsize 0 15))
-      (14 : (hax__autogenerated_refinement__BoundedUsize_BoundedUsize 0 15))
+    (2 : (hax__autogenerated_refinement__BoundedUsize.BoundedUsize 0 15))
+      (6 : (hax__autogenerated_refinement__BoundedUsize.BoundedUsize 0 15))
+      (10 : (hax__autogenerated_refinement__BoundedUsize.BoundedUsize 0 15))
+      (14 : (hax__autogenerated_refinement__BoundedUsize.BoundedUsize 0 15))
       state);
-  let (state : (Vector u32 16)) ← pure
+  let (state : (RustArray UInt32 16)) ← pure
     (← chacha20_quarter_round
-    (3 : (hax__autogenerated_refinement__BoundedUsize_BoundedUsize 0 15))
-      (7 : (hax__autogenerated_refinement__BoundedUsize_BoundedUsize 0 15))
-      (11 : (hax__autogenerated_refinement__BoundedUsize_BoundedUsize 0 15))
-      (15 : (hax__autogenerated_refinement__BoundedUsize_BoundedUsize 0 15))
+    (3 : (hax__autogenerated_refinement__BoundedUsize.BoundedUsize 0 15))
+      (7 : (hax__autogenerated_refinement__BoundedUsize.BoundedUsize 0 15))
+      (11 : (hax__autogenerated_refinement__BoundedUsize.BoundedUsize 0 15))
+      (15 : (hax__autogenerated_refinement__BoundedUsize.BoundedUsize 0 15))
       state);
-  let (state : (Vector u32 16)) ← pure
+  let (state : (RustArray UInt32 16)) ← pure
     (← chacha20_quarter_round
-    (0 : (hax__autogenerated_refinement__BoundedUsize_BoundedUsize 0 15))
-      (5 : (hax__autogenerated_refinement__BoundedUsize_BoundedUsize 0 15))
-      (10 : (hax__autogenerated_refinement__BoundedUsize_BoundedUsize 0 15))
-      (15 : (hax__autogenerated_refinement__BoundedUsize_BoundedUsize 0 15))
+    (0 : (hax__autogenerated_refinement__BoundedUsize.BoundedUsize 0 15))
+      (5 : (hax__autogenerated_refinement__BoundedUsize.BoundedUsize 0 15))
+      (10 : (hax__autogenerated_refinement__BoundedUsize.BoundedUsize 0 15))
+      (15 : (hax__autogenerated_refinement__BoundedUsize.BoundedUsize 0 15))
       state);
-  let (state : (Vector u32 16)) ← pure
+  let (state : (RustArray UInt32 16)) ← pure
     (← chacha20_quarter_round
-    (1 : (hax__autogenerated_refinement__BoundedUsize_BoundedUsize 0 15))
-      (6 : (hax__autogenerated_refinement__BoundedUsize_BoundedUsize 0 15))
-      (11 : (hax__autogenerated_refinement__BoundedUsize_BoundedUsize 0 15))
-      (12 : (hax__autogenerated_refinement__BoundedUsize_BoundedUsize 0 15))
+    (1 : (hax__autogenerated_refinement__BoundedUsize.BoundedUsize 0 15))
+      (6 : (hax__autogenerated_refinement__BoundedUsize.BoundedUsize 0 15))
+      (11 : (hax__autogenerated_refinement__BoundedUsize.BoundedUsize 0 15))
+      (12 : (hax__autogenerated_refinement__BoundedUsize.BoundedUsize 0 15))
       state);
-  let (state : (Vector u32 16)) ← pure
+  let (state : (RustArray UInt32 16)) ← pure
     (← chacha20_quarter_round
-    (2 : (hax__autogenerated_refinement__BoundedUsize_BoundedUsize 0 15))
-      (7 : (hax__autogenerated_refinement__BoundedUsize_BoundedUsize 0 15))
-      (8 : (hax__autogenerated_refinement__BoundedUsize_BoundedUsize 0 15))
-      (13 : (hax__autogenerated_refinement__BoundedUsize_BoundedUsize 0 15))
+    (2 : (hax__autogenerated_refinement__BoundedUsize.BoundedUsize 0 15))
+      (7 : (hax__autogenerated_refinement__BoundedUsize.BoundedUsize 0 15))
+      (8 : (hax__autogenerated_refinement__BoundedUsize.BoundedUsize 0 15))
+      (13 : (hax__autogenerated_refinement__BoundedUsize.BoundedUsize 0 15))
       state);
   (← chacha20_quarter_round
-  (3 : (hax__autogenerated_refinement__BoundedUsize_BoundedUsize 0 15))
-    (4 : (hax__autogenerated_refinement__BoundedUsize_BoundedUsize 0 15))
-    (9 : (hax__autogenerated_refinement__BoundedUsize_BoundedUsize 0 15))
-    (14 : (hax__autogenerated_refinement__BoundedUsize_BoundedUsize 0 15))
+  (3 : (hax__autogenerated_refinement__BoundedUsize.BoundedUsize 0 15))
+    (4 : (hax__autogenerated_refinement__BoundedUsize.BoundedUsize 0 15))
+    (9 : (hax__autogenerated_refinement__BoundedUsize.BoundedUsize 0 15))
+    (14 : (hax__autogenerated_refinement__BoundedUsize.BoundedUsize 0 15))
     state)
 
-def chacha20_rounds (state : (Vector u32 16)) : Result (Vector u32 16) := do
-  let (st : (Vector u32 16)) ← pure state;
-  let (st : (Vector u32 16)) ← pure
-    (← hax_folds_fold_range
+def chacha20_rounds (state : (RustArray UInt32 16))
+  : Result (RustArray UInt32 16) := do
+  let (st : (RustArray UInt32 16)) ← pure state;
+  let (st : (RustArray UInt32 16)) ← pure
+    (← hax.folds.fold_range
     0
       10
-      (fun (st : (Vector u32 16)) (_ : i32)=> do true)
+      (fun (st : (RustArray UInt32 16)) (_ : Int32) => do true)
       st
-      (fun (st : (Vector u32 16)) (_i : i32)=> do
+      (fun (st : (RustArray UInt32 16)) (_i : Int32) => do
         (← chacha20_double_round st)));
   st
 
-def chacha20_core (ctr : u32) (st0 : (Vector u32 16))
-  : Result (Vector u32 16) := do
-  let (state : (Vector u32 16)) ← pure st0;
-  let (state : (Vector u32 16)) ← pure
-    (← hax_monomorphized_update_at_update_at_usize
+def chacha20_core (ctr : UInt32) (st0 : (RustArray UInt32 16))
+  : Result (RustArray UInt32 16) := do
+  let (state : (RustArray UInt32 16)) ← pure st0;
+  let (state : (RustArray UInt32 16)) ← pure
+    (← hax.monomorphized_update_at.update_at_usize
     state
       12
-      (← num__8_impl_wrapping_add (← ops_index_Index_index state 12) ctr));
-  let (k : (Vector u32 16)) ← pure (← chacha20_rounds state);
-  (← hacspec_helper_add_state state k)
+      (← num._8_impl.wrapping_add (← ops.index.Index.index state 12) ctr));
+  let (k : (RustArray UInt32 16)) ← pure (← chacha20_rounds state);
+  (← hacspec_helper.add_state state k)
 
-def chacha20_init (key : (Vector u8 32)) (iv : (Vector u8 12)) (ctr : u32)
-  : Result (Vector u32 16) := do
-  let (key_u32 : (Vector u32 8)) ← pure
-    (← hacspec_helper_to_le_u32s_8 (← unsize key));
-  let (iv_u32 : (Vector u32 3)) ← pure
-    (← hacspec_helper_to_le_u32s_3 (← unsize iv));
+def chacha20_init
+  (key : (RustArray UInt8 32)) (iv : (RustArray UInt8 12)) (ctr : UInt32)
+  : Result (RustArray UInt32 16) := do
+  let ((key_u32 : (RustArray UInt32 8)) : (RustArray UInt32 8)) ← pure
+    (← hacspec_helper.to_le_u32s_8 (← unsize key));
+  let ((iv_u32 : (RustArray UInt32 3)) : (RustArray UInt32 3)) ← pure
+    (← hacspec_helper.to_le_u32s_3 (← unsize iv));
   #v[1634760805,
     857760878,
     2036477234,
     1797285236,
-    (← ops_index_Index_index key_u32 0),
-    (← ops_index_Index_index key_u32 1),
-    (← ops_index_Index_index key_u32 2),
-    (← ops_index_Index_index key_u32 3),
-    (← ops_index_Index_index key_u32 4),
-    (← ops_index_Index_index key_u32 5),
-    (← ops_index_Index_index key_u32 6),
-    (← ops_index_Index_index key_u32 7),
+    (← ops.index.Index.index key_u32 0),
+    (← ops.index.Index.index key_u32 1),
+    (← ops.index.Index.index key_u32 2),
+    (← ops.index.Index.index key_u32 3),
+    (← ops.index.Index.index key_u32 4),
+    (← ops.index.Index.index key_u32 5),
+    (← ops.index.Index.index key_u32 6),
+    (← ops.index.Index.index key_u32 7),
     ctr,
-    (← ops_index_Index_index iv_u32 0),
-    (← ops_index_Index_index iv_u32 1),
-    (← ops_index_Index_index iv_u32 2)]
+    (← ops.index.Index.index iv_u32 0),
+    (← ops.index.Index.index iv_u32 1),
+    (← ops.index.Index.index iv_u32 2)]
 
-def chacha20_key_block (state : (Vector u32 16)) : Result (Vector u8 64) := do
-  let (state : (Vector u32 16)) ← pure (← chacha20_core 0 state);
-  (← hacspec_helper_u32s_to_le_bytes state)
+def chacha20_key_block (state : (RustArray UInt32 16))
+  : Result (RustArray UInt8 64) := do
+  let (state : (RustArray UInt32 16)) ← pure (← chacha20_core 0 state);
+  (← hacspec_helper.u32s_to_le_bytes state)
 
-def chacha20_key_block0 (key : (Vector u8 32)) (iv : (Vector u8 12))
-  : Result (Vector u8 64) := do
-  let (state : (Vector u32 16)) ← pure (← chacha20_init key iv 0);
+def chacha20_key_block0 (key : (RustArray UInt8 32)) (iv : (RustArray UInt8 12))
+  : Result (RustArray UInt8 64) := do
+  let (state : (RustArray UInt32 16)) ← pure (← chacha20_init key iv 0);
   (← chacha20_key_block state)
 
 def chacha20_encrypt_block
-    (st0 : (Vector u32 16)) (ctr : u32) (plain : (Vector u8 64))
-  : Result (Vector u8 64) := do
-  let (st : (Vector u32 16)) ← pure (← chacha20_core ctr st0);
-  let (pl : (Vector u32 16)) ← pure
-    (← hacspec_helper_to_le_u32s_16 (← unsize plain));
-  let (encrypted : (Vector u32 16)) ← pure (← hacspec_helper_xor_state st pl);
-  (← hacspec_helper_u32s_to_le_bytes encrypted)
+  (st0 : (RustArray UInt32 16)) (ctr : UInt32) (plain : (RustArray UInt8 64))
+  : Result (RustArray UInt8 64) := do
+  let (st : (RustArray UInt32 16)) ← pure (← chacha20_core ctr st0);
+  let ((pl : (RustArray UInt32 16)) : (RustArray UInt32 16)) ← pure
+    (← hacspec_helper.to_le_u32s_16 (← unsize plain));
+  let (encrypted : (RustArray UInt32 16)) ← pure
+    (← hacspec_helper.xor_state st pl);
+  (← hacspec_helper.u32s_to_le_bytes encrypted)
 
-def __requires (st0 : (Vector u32 16)) (ctr : u32) (plain : (Array u8))
+def _.requires
+  (st0 : (RustArray UInt32 16)) (ctr : UInt32) (plain : (RustSlice UInt8))
   : Result Bool := do
-  (← hax_machine_int_le (← slice_impl_len u8 plain) 64)
+  (← hax.machine_int.le (← slice.impl.len UInt8 plain) 64)
 
 def chacha20_encrypt_last
-    (st0 : (Vector u32 16)) (ctr : u32) (plain : (Array u8))
-  : Result (vec_Vec u8 alloc_Global) := do
-  let (b : (Vector u8 64)) ← pure (← hax_repeat 0 64);
-  let (b : (Vector u8 64)) ← pure (← hacspec_helper_update_array b plain);
-  let (b : (Vector u8 64)) ← pure (← chacha20_encrypt_block st0 ctr b);
-  (← slice_impl_to_vec u8
-  (← ops_index_Index_index
+  (st0 : (RustArray UInt32 16)) (ctr : UInt32) (plain : (RustSlice UInt8))
+  : Result (vec.Vec UInt8 alloc.Global) := do
+  let ((b : (RustArray UInt8 64)) : (RustArray UInt8 64)) ← pure
+    (← hax.repeat 0 64);
+  let (b : (RustArray UInt8 64)) ← pure (← hacspec_helper.update_array b plain);
+  let (b : (RustArray UInt8 64)) ← pure (← chacha20_encrypt_block st0 ctr b);
+  (← slice.impl.to_vec UInt8
+  (← ops.index.Index.index
     b
-      (constr_ops_range_Range
-        (ops_range_Range_start := 0)
-        (ops_range_Range_end := (← slice_impl_len u8 plain)))))
+      (ops.range.Range.mk
+      (_start := 0) (_end := (← slice.impl.len UInt8 plain)))))
 
-def chacha20_update (st0 : (Vector u32 16)) (m : (Array u8))
-  : Result (vec_Vec u8 alloc_Global) := do
-  let (blocks_out : (vec_Vec u8 alloc_Global)) ← pure
-    (← vec_impl_new u8 hax_Tuple0);
-  let (num_blocks : usize) ← pure
-    (← hax_machine_int_div (← slice_impl_len u8 m) 64);
-  let (remainder_len : usize) ← pure
-    (← hax_machine_int_rem (← slice_impl_len u8 m) 64);
-  let (blocks_out : (vec_Vec u8 alloc_Global)) ← pure
-    (← hax_folds_fold_range
+def chacha20_update (st0 : (RustArray UInt32 16)) (m : (RustSlice UInt8))
+  : Result (vec.Vec UInt8 alloc.Global) := do
+  let (blocks_out : (vec.Vec UInt8 alloc.Global)) ← pure
+    (← vec.impl.new UInt8 hax.Tuple0);
+  let (num_blocks : USize) ← pure (← (← slice.impl.len UInt8 m) /? 64);
+  let (remainder_len : USize) ← pure (← (← slice.impl.len UInt8 m) %? 64);
+  let (blocks_out : (vec.Vec UInt8 alloc.Global)) ← pure
+    (← hax.folds.fold_range
     0
       num_blocks
-      (fun (blocks_out : (vec_Vec u8 alloc_Global)) (_ : usize)=> do true)
+      (fun (blocks_out : (vec.Vec UInt8 alloc.Global)) (_ : USize) => do true)
       blocks_out
-      (fun (blocks_out : (vec_Vec u8 alloc_Global)) (i : usize)=> do
-        let (b : (Vector u8 64)) ← pure
+      (fun (blocks_out : (vec.Vec UInt8 alloc.Global)) (i : USize) => do
+        let (b : (RustArray UInt8 64)) ← pure
           (← chacha20_encrypt_block
           st0
-            (← hax_cast_op i)
-            (← result_impl_unwrap (Vector u8 64) array_TryFromSliceError
-            (← convert_TryInto_try_into
-              (← ops_index_Index_index
+            (← hax.cast_op i)
+            (← result.impl.unwrap (RustArray UInt8 64) array.TryFromSliceError
+            (← convert.TryInto.try_into
+              (← ops.index.Index.index
                 m
-                  (constr_ops_range_Range
-                    (ops_range_Range_start := (← hax_machine_int_mul 64 i))
-                    (ops_range_Range_end := (← (← hax_machine_int_mul 64 i) +?
-                    64)))))));
-        let (_ : hax_Tuple0) ← pure
+                  (ops.range.Range.mk
+                  (_start := (← 64 *? i)) (_end := (← (← 64 *? i) +? 64)))))));
+        let (_ : hax.Tuple0) ← pure
           (← assume
-          (← prop_constructors_from_bool
-            (← hax_machine_int_eq
-              (← vec__1_impl_len u8 alloc_Global blocks_out)
-                (← hax_machine_int_mul i 64))));
-        let (blocks_out : (vec_Vec u8 alloc_Global)) ← pure
-          (← vec__2_impl_extend_from_slice u8 alloc_Global
+          (← prop.constructors.from_bool
+            (← hax.machine_int.eq
+              (← vec._1_impl.len UInt8 alloc.Global blocks_out)
+                (← i *? 64))));
+        let (blocks_out : (vec.Vec UInt8 alloc.Global)) ← pure
+          (← vec._2_impl.extend_from_slice UInt8 alloc.Global
           blocks_out
             (← unsize b));
         blocks_out));
-  let (_ : hax_Tuple0) ← pure
+  let (_ : hax.Tuple0) ← pure
     (← assume
-    (← prop_constructors_from_bool
-      (← hax_machine_int_eq
-        (← vec__1_impl_len u8 alloc_Global blocks_out)
-          (← hax_machine_int_mul num_blocks 64))));
-  let (blocks_out : (vec_Vec u8 alloc_Global)) ←
-    if (← hax_machine_int_ne remainder_len 0)
+    (← prop.constructors.from_bool
+      (← hax.machine_int.eq
+        (← vec._1_impl.len UInt8 alloc.Global blocks_out)
+          (← num_blocks *? 64))));
+  let (blocks_out : (vec.Vec UInt8 alloc.Global)) ←
+    if (← hax.machine_int.ne remainder_len 0)
     then
-      let (b : (vec_Vec u8 alloc_Global)) ← pure
+      let (b : (vec.Vec UInt8 alloc.Global)) ← pure
         (← chacha20_encrypt_last
         st0
-          (← hax_cast_op num_blocks)
-          (← ops_index_Index_index
+          (← hax.cast_op num_blocks)
+          (← ops.index.Index.index
           m
-            (constr_ops_range_Range
-              (ops_range_Range_start := (← hax_machine_int_mul 64 num_blocks))
-              (ops_range_Range_end := (← slice_impl_len u8 m)))));
-      let (blocks_out : (vec_Vec u8 alloc_Global)) ← pure
-        (← vec__2_impl_extend_from_slice u8 alloc_Global
+            (ops.range.Range.mk
+            (_start := (← 64 *? num_blocks))
+            (_end := (← slice.impl.len UInt8 m)))));
+      let (blocks_out : (vec.Vec UInt8 alloc.Global)) ← pure
+        (← vec._2_impl.extend_from_slice UInt8 alloc.Global
         blocks_out
-          (← ops_deref_Deref_deref b));
-      blocks_out
-    else blocks_out;
+          (← ops.deref.Deref.deref b));
+      pure blocks_out
+    else pure blocks_out;
   blocks_out
 
 def chacha20
-    (m : (Array u8)) (key : (Vector u8 32)) (iv : (Vector u8 12)) (ctr : u32)
-  : Result (vec_Vec u8 alloc_Global) := do
-  let (state : (Vector u32 16)) ← pure (← chacha20_init key iv ctr);
+  (m : (RustSlice UInt8)) (key : (RustArray UInt8 32)) (iv : (RustArray
+  UInt8
+  12)) (ctr : UInt32) : Result (vec.Vec UInt8 alloc.Global) := do
+  let (state : (RustArray UInt32 16)) ← pure (← chacha20_init key iv ctr);
   (← chacha20_update state m)
-
 
 -- Theorems
 
 @[spec]
-theorem hacspec_helper_add_state_spec (state : (Vector u32 16)) (other : (Vector u32 16)) :
+theorem hacspec_helper.add_state_spec (state : (Vector u32 16)) (other : (Vector u32 16)) :
   ⦃ ⌜ True ⌝ ⦄
-  (hacspec_helper_add_state state other)
+  (hacspec_helper.add_state state other)
   ⦃ ⇓ _ => True ⦄ := by
-  mvcgen [hacspec_helper_add_state]
+  mvcgen [hacspec_helper.add_state]
   <;> try apply SPred.pure_intro
   <;> simp [Vector.size] at *
   <;> cases System.Platform.numBits_eq with
@@ -429,16 +433,15 @@ theorem hacspec_helper_add_state_spec (state : (Vector u32 16)) (other : (Vector
       omega
 
 @[spec]
-theorem hacspec_helper_to_le_u32s_16_spec bytes :
+theorem hacspec_helper.to_le_u32s_16_spec bytes :
   bytes.size = 64 →
   ⦃ ⌜ True ⌝ ⦄
-  (hacspec_helper_to_le_u32s_16 bytes)
+  (hacspec_helper.to_le_u32s_16 bytes)
   ⦃ ⇓ _ => True ⦄ := by
   intro
   open SpecNat in
-  mvcgen [hacspec_helper_to_le_u32s_16,
-    convert_TryInto_try_success_spec,
-    result_impl_unwrap_spec]
+  mvcgen [hacspec_helper.to_le_u32s_16,
+    result.impl.unwrap.spec]
   <;> (try apply SPred.pure_intro)
   all_goals simp [USize.size, Vector.size] at *
   any_goals subst_vars
@@ -452,17 +455,16 @@ theorem hacspec_helper_to_le_u32s_16_spec bytes :
 
 
 @[spec]
-theorem hacspec_helper_to_le_u32s_3_spec bytes :
+theorem hacspec_helper.to_le_u32s_3_spec bytes :
   bytes.size = 12 →
   ⦃ ⌜ True ⌝ ⦄
-  (hacspec_helper_to_le_u32s_3 bytes)
+  (hacspec_helper.to_le_u32s_3 bytes)
   ⦃ ⇓ _ => True ⦄ := by
   intros
   open SpecNat in
-  mvcgen [hacspec_helper_to_le_u32s_3,
-    convert_TryInto_try_success_spec,
-    result_impl_unwrap_spec]
-  all_goals simp [USize.size, Vector.size] at *
+  mvcgen [hacspec_helper.to_le_u32s_3,
+    result.impl.unwrap.spec]
+  all_goals simp [USize.size, RustArray, Vector.size] at *
   any_goals subst_vars
   all_goals try simp [USize.le_iff_toNat_le]
   all_goals try (cases System.Platform.numBits_eq with
@@ -473,17 +475,17 @@ theorem hacspec_helper_to_le_u32s_3_spec bytes :
       omega ; done )
 
 
+
 @[spec]
-theorem hacspec_helper_to_le_u32s_8_spec (bytes : (Array u8)) :
+theorem hacspec_helper.to_le_u32s_8_spec (bytes : (Array u8)) :
   bytes.size = 32 →
   ⦃ ⌜ True ⌝ ⦄
-  ( hacspec_helper_to_le_u32s_8 bytes )
+  ( hacspec_helper.to_le_u32s_8 bytes )
   ⦃ ⇓ _ => True ⦄ := by
   intros
   open SpecNat in
-  mvcgen [hacspec_helper_to_le_u32s_8,
-    convert_TryInto_try_success_spec,
-    result_impl_unwrap_spec]
+  mvcgen [hacspec_helper.to_le_u32s_8,
+    result.impl.unwrap.spec]
   all_goals simp [USize.size, Vector.size] at *
   any_goals subst_vars
   all_goals try simp [USize.le_iff_toNat_le]
@@ -495,16 +497,15 @@ theorem hacspec_helper_to_le_u32s_8_spec (bytes : (Array u8)) :
       omega ; done )
 
 @[spec]
-theorem hacspec_helper_u32s_to_le_bytes_spec (state : (Vector u32 16)) :
+theorem hacspec_helper.u32s_to_le_bytes_spec (state : (Vector u32 16)) :
   ⦃ ⌜ True ⌝ ⦄
-  (hacspec_helper_u32s_to_le_bytes state)
+  (hacspec_helper.u32s_to_le_bytes state)
   ⦃ ⇓ _ => True ⦄ := by
   intros
   open SpecNat in
-  mvcgen [hacspec_helper_u32s_to_le_bytes,
-    convert_TryInto_try_success_spec,
-    result_impl_unwrap_spec,
-    num__8_impl_to_le_bytes]
+  mvcgen [hacspec_helper.u32s_to_le_bytes,
+    result.impl.unwrap.spec,
+    num._8_impl.to_le_bytes]
   all_goals simp [USize.size, Vector.size] at *
   any_goals subst_vars
   all_goals try simp [USize.toNat_ofNat'] at *
@@ -519,17 +520,15 @@ theorem hacspec_helper_u32s_to_le_bytes_spec (state : (Vector u32 16)) :
       omega ; done )
 
 @[spec]
-theorem hacspec_helper_xor_state_spec (state other: (Vector u32 16)) :
+theorem hacspec_helper.xor_state_spec (state other: (Vector u32 16)) :
   ⦃ ⌜ True ⌝ ⦄
-  (hacspec_helper_xor_state state other)
+  (hacspec_helper.xor_state state other)
   ⦃ ⇓ _ => True ⦄ := by
   intros
   open SpecNat in
-  mvcgen [hacspec_helper_xor_state,
-    convert_TryInto_try_success_spec,
-    result_impl_unwrap_spec,
-    hax_monomorphized_update_at_update_at_usize_spec,
-    num__8_impl_to_le_bytes]
+  mvcgen [hacspec_helper.xor_state,
+    result.impl.unwrap.spec,
+    num._8_impl.to_le_bytes]
   all_goals simp [USize.size, Vector.size, USize.le_iff_toNat_le] at *
   any_goals subst_vars
   all_goals try simp [USize.toNat_ofNat'] at *
@@ -542,18 +541,15 @@ theorem hacspec_helper_xor_state_spec (state other: (Vector u32 16)) :
 
 
 @[spec]
-theorem hacspec_helper_update_array_spec (a: (Vector u8 64)) (v: Array u8) :
+theorem hacspec_helper.update_array_spec (a: (Vector u8 64)) (v: Array u8) :
   v.size ≤ 64 →
   ⦃ ⌜ True ⌝ ⦄
-  (hacspec_helper_update_array a v)
+  (hacspec_helper.update_array a v)
   ⦃ ⇓ _ => True ⦄ := by
   intros
   open SpecNat in
-  mvcgen_step 24 [hacspec_helper_update_array,
-    convert_TryInto_try_success_spec,
-    result_impl_unwrap_spec,
-    hax_monomorphized_update_at_update_at_usize_spec,
-    num__8_impl_to_le_bytes]
+  mvcgen_step 24 [hacspec_helper.update_array,
+    result.impl.unwrap.spec]
   all_goals simp [USize.size, Vector.size, USize.le_iff_toNat_le, USize.lt_iff_toNat_lt] at *
   any_goals subst_vars
   all_goals try simp [USize.toNat_ofNat'] at *
@@ -568,9 +564,9 @@ theorem hacspec_helper_update_array_spec (a: (Vector u8 64)) (v: Array u8) :
 
 @[spec]
 theorem chacha20_line_spec
-    (a : (hax__autogenerated_refinement__BoundedUsize_BoundedUsize 0 15)) (b :
-    (hax__autogenerated_refinement__BoundedUsize_BoundedUsize 0 15)) (d :
-    (hax__autogenerated_refinement__BoundedUsize_BoundedUsize 0 15)) (s : u32)
+    (a : (hax__autogenerated_refinement__BoundedUsize.BoundedUsize 0 15)) (b :
+    (hax__autogenerated_refinement__BoundedUsize.BoundedUsize 0 15)) (d :
+    (hax__autogenerated_refinement__BoundedUsize.BoundedUsize 0 15)) (s : u32)
     (m : (Vector u32 16)) :
   ⦃ a.toNat ≤ 15 ∧ b.toNat ≤ 15 ∧ d.toNat ≤ 15 ⦄
   (chacha20_line a b d s m )
@@ -586,8 +582,7 @@ theorem chacha20_quarter_round_spec a b c d state:
   mintro ⟨ha, hb, hc, hd⟩
   mvcgen [chacha20_quarter_round,
           chacha20_line,
-          hax_machine_int_bitxor,
-          num__8_impl_rotate_left,
+          hax.machine_int.bitxor,
           Result.ofOption,
           ] <;> try (simp;omega;done)
 
@@ -613,7 +608,7 @@ theorem chacha20_core_spec ctr state :
   (chacha20_core ctr state)
   ⦃ ⇓ _ => True ⦄
 := by
-  mvcgen [chacha20_core, ops_index_Index_index, GetElemResult, Result.ofOption, hax_monomorphized_update_at_update_at_usize]
+  mvcgen [chacha20_core,  GetElemResult, Result.ofOption]
   simp [Vector.size] at *
 
 
@@ -652,7 +647,7 @@ theorem chacha20_encrypt_last_spec (st0 : (Vector u32 16)) (ctr : u32) (plain : 
   ( chacha20_encrypt_last st0 ctr plain)
   ⦃ ⇓ _ => True ⦄
 := by
-  mvcgen [chacha20_encrypt_last, slice_impl_len]
+  mvcgen [chacha20_encrypt_last, slice.impl.len]
   <;> (try apply SPred.pure_intro)
   <;> (try simp)
   simp [Vector.size, USize.le_iff_toNat_le] at *
@@ -672,10 +667,9 @@ theorem chacha20_update_spec (st0 : (Vector u32 16)) (m : (Array u8)) :
 := by
   open SpecNat in
   mvcgen [chacha20_update,
-    vec_impl_new, slice_impl_len,
-    convert_TryInto_try_success_spec,
-    result_impl_unwrap_spec,
-    vec__1_impl_len,
+    vec.impl.new, slice.impl.len,
+    result.impl.unwrap.spec,
+    vec._1_impl.len,
     ] <;> subst_vars
   all_goals simp [Array.size_extract, USize.eq_iff_toBitVec_eq, BitVec.toNat_eq, USize.size, USize.le_iff_toNat_le ] at *
   all_goals try cases System.Platform.numBits_eq with
